Classes/Monad/MonadExcept.v
@@ -1,0 +1,20 @@
+Require Export Base.
+Require Import Classes.Applicative.
+Require Import Classes.Monad.
+Require Import Classes.Monad.MonadFail.
+
+Implicit Type M : Type → Type.
+Implicit Type A : Type.
+
+Class MonadExcept M `{MonadFail M} := {
+  catch : forall {A}, M A -> M A -> M A;
+  catch_left : forall {A} (x : M A), catch fail x = x;
+  catch_right : forall {A} (x : M A), catch x fail = x;
+  catch_assoc : ∀ {A} (x y z: M A),
+    catch x (catch y z) = catch (catch x y) z;
+  catch_pure : ∀ {A} (x : M A) (a : A),
+    catch (pure a) x = pure a;
+}.
+Arguments catch : simpl never.
+
+Hint Rewrite @catch_left @catch_right @catch_pure : soundness.
