Classes/Monad/MonadFail.v
@@ -1,0 +1,13 @@
+Require Export Base.
+Require Import Classes.Monad.
+Require Import Classes.Applicative.
+
+Class MonadFail M `{Monad M} : Type := {
+  fail {A : Type} : M A;
+  fail_left: ∀ {A B} (m : A → M B), (@fail A) >>= m = fail;
+}.
+Arguments fail : simpl never.
+Hint Rewrite @fail_left : soundness.
+
+Definition guard {M} `{MonadFail M} : bool → M unit := 
+  λ b, if b then skip else fail.
